Specialize FinMap to threads

src/Helpers/FinMap.v
@@ -1,470 +1,483 @@
-(* a finite partial map *)
+(* representation of thread states as a a finite partial map, with an explicit
+bound beyond which no more threads are mapped *)
 
 Require Import Arith.
 Require Import Omega.
 Require Import FunctionalExtensionality.
 Require Import ProofIrrelevance.
+Require Import Helpers.Helpers.
+
+Require Import ConcurProc.
 
 Set Implicit Arguments.
 
-Module Map.
-  Section Map.
-    Notation A := nat.
-    Infix "==" := Nat.eq_dec (no associativity, at level 30).
+Section Map.
+  Notation A := nat.
 
-    Variable V:Type.
+  Variable Op : Type -> Type.
+  Notation V := (maybe_proc Op).
 
-    Local Record t :=
-      { get :> A -> option V;
-        max : nat;
-        mapping_finite : forall a, max < a -> get a = None;
-        max_minimal : (get max <> None) \/ max = 0 }.
+  Local Record threads_state :=
+    { thread_get :> A -> V;
+      thread_max : nat;
+      mapping_finite : forall a, thread_max < a -> thread_get a = NoProc;
+      thread_max_minimal : (thread_get thread_max <> NoProc) \/ thread_max = 0 }.
 
-    Hint Extern 4 (_ < _) => omega.
-    Hint Resolve mapping_finite.
-    Hint Extern 2 (_ <> _) => congruence.
-    Hint Extern 2 (_ = _ -> False) => congruence.
-    Hint Resolve max_minimal.
+  Notation t := threads_state.
 
-    Fixpoint lower_mapping (x:t) n : A :=
-      match n with
-      | 0 => 0
-      | S n' => match x n' with
-               | Some _ => n'
-               | None => lower_mapping x n'
-               end
-      end.
+  Hint Extern 4 (_ < _) => omega.
+  Hint Resolve mapping_finite.
+  Hint Extern 2 (_ <> _) => congruence.
+  Hint Extern 2 (_ = _ -> False) => congruence.
+  Hint Resolve thread_max_minimal.
 
-    Theorem lower_mapping_smaller : forall x n,
-        lower_mapping x n < n \/ n = 0.
-    Proof.
-      induction n; simpl; auto.
-      destruct (x n); intuition auto.
-      subst; auto.
-    Qed.
+  Fixpoint lower_mapping (x:threads_state) n : A :=
+    match n with
+    | 0 => 0
+    | S n' => match x n' with
+             | Proc _ => n'
+             | NoProc => lower_mapping x n'
+             end
+    end.
 
-    Theorem lower_mapping_not_none : forall (x:t) n,
-        x (lower_mapping x n) <> None \/
-        lower_mapping x n = 0.
-    Proof.
-      induction n; simpl; auto.
-      destruct_with_eqn (x n); intuition auto.
-    Qed.
-
-    Theorem lower_mapping_maximal : forall x n,
-        forall a, lower_mapping x n < a -> a < n -> x a = None.
-    Proof.
-      intros.
-      induction n; simpl in *; intros.
-      exfalso; omega.
-      destruct_with_eqn (x n); auto.
-      destruct (a == n); subst; auto.
-    Qed.
-
-    Definition upd (x:t) (a:A) (v:option V) : t.
-      refine {| get :=
-                  fun a' => if a == a' then v else x a';
-                max :=
-                  if lt_dec (max x) a then
-                    (* modification past current end *)
-                    match v with
-                    | Some _ => a
-                    | None => max x (* no-op *)
-                    end else
-                    match v with
-                    | Some _ => max x
-                    | None => (* deleting from the middle; might need to lower max *)
-                        if a == max x then
-                          lower_mapping x (max x) else
-                          max x
-                    end|};
-        intros.
-      - destruct (lt_dec (max x) a), (a == a0), v; subst; try omega; auto.
-        destruct (a == max x); subst; auto.
-        destruct (lt_dec a0 (max x)); auto.
-        apply lower_mapping_maximal with (n := max x); auto.
-      - destruct (lt_dec (max x) a), v; subst;
-          repeat match goal with
-                 | |- context[if ?a == ?b then _ else _] => destruct (a == b)
-                 end; subst; try omega; auto.
-        destruct (lower_mapping_smaller x (max x)); try omega.
-        rewrite H; simpl; auto.
-        destruct (lower_mapping_not_none x (max x)); auto.
-    Defined.
-
-    Theorem t_ext_eq : forall (x y:t),
-        (forall a, x a = y a) ->
-        x = y.
-    Proof.
-      intros.
-      destruct x as [x x_max mapping_finite_x max_minimal_x].
-      destruct y as [y y_max mapping_finite_y max_minimal_y].
-      simpl in *.
-      assert (x = y).
-      extensionality a; auto.
-      subst y.
-      clear H.
-      assert (x_max = y_max). { (* the main proof *)
-        destruct max_minimal_x, max_minimal_y; subst; auto.
-        - assert (~x_max < y_max) by (intro; eauto).
-          assert (~y_max < x_max) by (intro; eauto).
-          omega.
-        - specialize (mapping_finite_y x_max).
-          destruct x_max; auto.
-          exfalso; auto.
-        - specialize (mapping_finite_x y_max).
-          destruct y_max; auto.
-          exfalso; auto.
-      }
-      subst.
-      f_equal; auto using proof_irrelevance.
-    Qed.
-
-    Ltac t :=
-      intros;
-      try lazymatch goal with
-          | |- @eq t _ _ => apply t_ext_eq; intros
-          end;
-      simpl;
-      repeat match goal with
-             | [ |- context[?a == ?a' ] ] =>
-               destruct (a == a')
-             | _ => congruence
-             end.
-
-    Theorem upd_eq : forall x a v,
-        upd x a v a = v.
-    Proof.
-      t.
-    Qed.
-
-    Theorem upd_ne: forall (x:t) a a' v,
-        a <> a' ->
-        upd x a v a' = x a'.
-    Proof.
-      t.
-    Qed.
-
-    Theorem upd_upd_eq : forall x a v v',
-        upd (upd x a v) a v' = upd x a v'.
-    Proof.
-      t.
-    Qed.
-
-    Theorem upd_ne_comm : forall (x:t) a a' v v',
-        a <> a' ->
-        upd (upd x a v) a' v' = upd (upd x a' v') a v.
-    Proof.
-      t.
-    Qed.
-
-    Theorem upd_same_eq : forall (x:t) a v,
-        x a = v ->
-        upd x a v = x.
-    Proof.
-      t.
-    Qed.
-
-    Theorem upd_max_bound : forall (x:t) a v,
-        a <= max x ->
-        max (upd x a v) <= max x.
-    Proof.
-      simpl; intros.
-      generalize dependent (max x); intros m **.
-      destruct (lt_dec m a).
-      destruct v; auto.
-      destruct v; auto.
-      destruct (a == m); subst; auto.
-      destruct (lower_mapping_smaller x m); subst; auto.
-      omega.
-    Qed.
-
-    Theorem upd_max_extend : forall (x:t) a v,
-        a > max x ->
-        max (upd x a (Some v)) > max x.
-    Proof.
-      simpl; intros.
-      generalize dependent (max x); intros m **.
-      destruct (lt_dec m a); auto.
-    Qed.
-
-    Theorem upd_max_extend_bound : forall (x:t) a v,
-        a >= max x ->
-        max (upd x a v) <= a.
-    Proof.
-      simpl; intros.
-      generalize dependent (max x); intros m **.
-      destruct (lt_dec m a); auto.
-      destruct v; auto; try omega.
-      destruct v; auto; try omega.
-      destruct (a == m); subst; auto.
-      destruct (lower_mapping_smaller x m); subst; auto.
-      omega.
-    Qed.
-
-    Theorem upd_max_shrink : forall (x:t) a,
-        max (upd x a None) <= max x.
-    Proof.
-      simpl; intros.
-      generalize dependent (max x); intros m **.
-      destruct (lt_dec m a); auto.
-      destruct (a == m); subst; auto.
-      destruct (lower_mapping_smaller x m); subst; auto.
-      omega.
-    Qed.
-
-    Theorem upd_unchanged : forall (x:t) a v,
-        a <= max x ->
-        max (upd x a (Some v)) = max x.
-    Proof.
-    Abort.
-
-    Theorem past_max_empty : forall (x:t),
-        x (1 + max x) = None.
-    Proof.
-      intros.
-      apply mapping_finite; omega.
-    Qed.
-
-    Definition empty : t.
-      refine {| get := fun _ => None;
-                max := 0; |}; auto.
-    Defined.
-
-    Theorem empty_is_empty : forall a,
-        empty a = None.
-    Proof.
-      simpl; auto.
-    Qed.
-
-    Theorem empty_not_some : forall a v,
-        ~empty a = Some v.
-    Proof.
-      simpl; auto.
-    Qed.
-
-    Theorem empty_unique : forall (x:t),
-        (forall a, x a = None) ->
-        x = empty.
-    Proof.
-      t.
-    Qed.
-
-    Theorem empty_max :
-      max empty = 0.
-    Proof.
-      t.
-    Qed.
-
-    Definition Forall (P: V -> Prop) (x:t) :=
-      forall a v, x a = Some v -> P v.
-
-    Theorem Forall_some : forall P x a v,
-        Forall P x ->
-        x a = Some v ->
-        P v.
-    Proof.
-      unfold Forall; eauto.
-    Qed.
-
-    Theorem empty_Forall : forall P,
-        Forall P empty.
-    Proof.
-      unfold Forall; intros.
-      apply empty_not_some in H; contradiction.
-    Qed.
-
-    Theorem Forall_upd_some : forall P x a v,
-        Forall P x ->
-        P v ->
-        Forall P (upd x a (Some v)).
-    Proof.
-      unfold Forall.
-      t.
-      destruct (a == a0); subst;
-        rewrite ?Map.upd_eq, ?Map.upd_ne in * by auto;
-        subst;
-        eauto.
-      congruence.
-    Qed.
-
-    Theorem Forall_forall : forall (P: V -> Prop) (x:t),
-        (forall a v, x a = Some v -> P v) ->
-        Forall P x.
-    Proof.
-      unfold Forall; eauto.
-    Qed.
-
-    Theorem Forall_upd_none : forall P x a,
-        Forall P x ->
-        Forall P (upd x a None).
-    Proof.
-      unfold Forall.
-      t.
-      destruct (a == a0); subst;
-        rewrite ?Map.upd_eq, ?Map.upd_ne in * by auto;
-        subst;
-        eauto.
-      congruence.
-    Qed.
-
-    Definition from_list (l: list V) : t.
-      refine {| get := fun a => List.nth_error l a;
-                max := length l - 1; |}.
-      intros.
-      apply List.nth_error_None; omega.
-      destruct_with_eqn (List.nth_error l (length l - 1)); eauto.
-      right.
-      apply List.nth_error_None in Heqo.
-      omega.
-    Defined.
-
-    Theorem from_list_get : forall l a,
-        from_list l a = List.nth_error l a.
-    Proof.
-      auto.
-    Qed.
-
-    Local Fixpoint _to_list (x:t) n : list (option V) :=
-      match n with
-      | 0 => nil
-      | S n' => _to_list x n' ++ (x n'::nil)
-      end.
-
-    Definition to_list (x:t) : list (option V) := _to_list x (1 + max x).
-
-    Lemma firstn_map : forall A B (f: A -> B) n (l: list A),
-        List.firstn n (List.map f l) = List.map f (List.firstn n l).
-    Proof.
-      induction n; simpl; intros; auto.
-      destruct l; simpl; eauto.
-      rewrite IHn; auto.
-    Qed.
-
-    Lemma nth_error_nil : forall A n,
-        List.nth_error (@nil A) n = None.
-    Proof.
-      induction n; simpl; eauto.
-    Qed.
-
-    (* TODO: prove this, just for fun (note that it is unused; conversion back
-    to lists is only for extraction purposes) *)
-    Lemma from_list__to_list : forall l n,
-        n <= length l ->
-        _to_list (from_list l) n = List.firstn n (List.map Some l).
-    Proof.
-      induction n; intros; auto.
-      cbn [_to_list get from_list].
-      rewrite IHn by omega.
-      rewrite ?firstn_map.
-      clear IHn.
-      fold (lt n (length l)) in H.
-    Admitted.
-
-    Theorem from_list_to_list : forall l,
-        0 < length l ->
-        to_list (from_list l) = List.map Some l.
-    Proof.
-      unfold to_list; intros.
-      unfold to_list.
-      rewrite from_list__to_list by (simpl; omega).
-      rewrite List.firstn_all2; auto.
-      rewrite List.map_length.
-      simpl; omega.
-    Qed.
-
-  End Map.
-
-  Theorem max_eq : forall V1 V2 (x1:t V1) (x2:t V2),
-      (forall a, x1 a = None <-> x2 a = None) ->
-      max x1 = max x2.
+  Theorem lower_mapping_smaller : forall x n,
+      lower_mapping x n < n \/ n = 0.
   Proof.
-    (* will do proof by symmetry *)
-    assert (forall V1 V2 (x1:t V1) (x2:t V2),
-               (forall a, x1 a = None <-> x2 a = None) ->
-               max x1 < max x2 -> False).
-    intros.
-    pose proof (@mapping_finite _ x1 (max x2) ltac:(omega)).
-    apply H in H1.
-    destruct (max_minimal x2); try congruence.
-    omega.
+    induction n; simpl; auto.
+    destruct (x n); intuition auto.
+    subst; auto.
+  Qed.
 
+  Theorem lower_mapping_not_none : forall (x:t) n,
+      x (lower_mapping x n) <> NoProc \/
+      lower_mapping x n = 0.
+  Proof.
+    induction n; simpl; auto.
+    destruct_with_eqn (x n); intuition auto.
+  Qed.
+
+  Theorem lower_mapping_thread_maximal : forall x n,
+      forall a, lower_mapping x n < a -> a < n -> x a = NoProc.
+  Proof.
     intros.
-    assert (forall a, x2 a = None <-> x1 a = None).
-    split; intuition auto.
-    apply H0; auto.
-    apply H0; auto.
-    pose proof (H _ _ x1 x2).
-    pose proof (H _ _ x2 x1).
-    intuition auto.
+    induction n; simpl in *; intros.
+    exfalso; omega.
+    destruct_with_eqn (x n); auto.
+    destruct (a == n); subst; auto.
+  Qed.
+
+  Definition thread_upd (x:t) (a:A) (v:V) : t.
+    refine {| thread_get :=
+                fun a' => if a == a' then v else x a';
+              thread_max :=
+                if lt_dec (thread_max x) a then
+                  (* modification past current end *)
+                  match v with
+                  | Proc _ => a
+                  | NoProc => thread_max x (* no-op *)
+                  end else
+                  match v with
+                  | Proc _ => thread_max x
+                  | NoProc => (* deleting from the middle; might need to lower thread_max *)
+                    if a == thread_max x then
+                      lower_mapping x (thread_max x) else
+                      thread_max x
+                  end|};
+      intros.
+    - destruct (lt_dec (thread_max x) a), (a == a0), v; subst; try omega; auto.
+      destruct (a == thread_max x); subst; auto.
+      destruct (lt_dec a0 (thread_max x)); auto.
+      apply lower_mapping_thread_maximal with (n := thread_max x); auto.
+    - destruct (lt_dec (thread_max x) a), v; subst;
+        repeat match goal with
+               | |- context[if ?a == ?b then _ else _] => destruct (a == b)
+               end; subst; try omega; auto.
+      destruct (lower_mapping_smaller x (thread_max x)); try omega.
+      rewrite H; simpl; auto.
+      destruct (lower_mapping_not_none x (thread_max x)); auto.
+  Defined.
+
+  Theorem thread_ext_eq : forall (x y:t),
+      (forall tid, x tid = y tid) ->
+      x = y.
+  Proof.
+    intros.
+    destruct x as [x x_thread_max mapping_finite_x thread_max_minimal_x].
+    destruct y as [y y_thread_max mapping_finite_y thread_max_minimal_y].
+    simpl in *.
+    assert (x = y).
+    extensionality tid; auto.
+    subst y.
+    clear H.
+    assert (x_thread_max = y_thread_max). { (* the main proof *)
+      destruct thread_max_minimal_x, thread_max_minimal_y; subst; auto.
+      - assert (~x_thread_max < y_thread_max) by (intro; eauto).
+        assert (~y_thread_max < x_thread_max) by (intro; eauto).
+        omega.
+      - specialize (mapping_finite_y x_thread_max).
+        destruct x_thread_max; auto.
+        exfalso; auto.
+      - specialize (mapping_finite_x y_thread_max).
+        destruct y_thread_max; auto.
+        exfalso; auto.
+    }
+    subst.
+    f_equal; auto using proof_irrelevance.
+  Qed.
+
+  Ltac t :=
+    intros;
+    try lazymatch goal with
+        | |- @eq t _ _ => apply thread_ext_eq; intros
+        end;
+    simpl;
+    repeat match goal with
+           | [ |- context[?a == ?a' ] ] =>
+             destruct (a == a')
+           | _ => congruence
+           end.
+
+  Theorem thread_upd_eq : forall x a v,
+      thread_upd x a v a = v.
+  Proof.
+    t.
+  Qed.
+
+  Theorem thread_upd_ne: forall (x:t) a a' v,
+      a <> a' ->
+      thread_upd x a v a' = x a'.
+  Proof.
+    t.
+  Qed.
+
+  Theorem thread_upd_thread_upd_eq : forall x a v v',
+      thread_upd (thread_upd x a v) a v' = thread_upd x a v'.
+  Proof.
+    t.
+  Qed.
+
+  Theorem thread_upd_ne_comm : forall (ts:t) tid tid' p p',
+      tid <> tid' ->
+      thread_upd (thread_upd ts tid p) tid' p' =
+      thread_upd (thread_upd ts tid' p') tid p.
+  Proof.
+    t.
+  Qed.
+
+  Theorem thread_upd_same_eq : forall (ts:t) tid p,
+      ts tid = p ->
+      thread_upd ts tid p = ts.
+  Proof.
+    t.
+  Qed.
+
+  Theorem thread_upd_thread_max_bound : forall (x:t) a v,
+      a <= thread_max x ->
+      thread_max (thread_upd x a v) <= thread_max x.
+  Proof.
+    simpl; intros.
+    generalize dependent (thread_max x); intros m **.
+    destruct (lt_dec m a).
+    destruct v; auto.
+    destruct v; auto.
+    destruct (a == m); subst; auto.
+    destruct (lower_mapping_smaller x m); subst; auto.
     omega.
   Qed.
 
-  Section Map_map.
+  Theorem thread_upd_thread_max_extend : forall (x:t) a T v,
+      a > thread_max x ->
+      thread_max (thread_upd x a (Proc (T:=T) v)) > thread_max x.
+  Proof.
+    simpl; intros.
+    generalize dependent (thread_max x); intros m **.
+    destruct (lt_dec m a); auto.
+  Qed.
 
-    Variable V1:Type.
-    Variable V2:Type.
-    Variable f:V1 -> V2.
+  Theorem thread_upd_thread_max_extend_bound : forall (x:t) a v,
+      a >= thread_max x ->
+      thread_max (thread_upd x a v) <= a.
+  Proof.
+    simpl; intros.
+    generalize dependent (thread_max x); intros m **.
+    destruct (lt_dec m a); auto.
+    destruct v; auto; try omega.
+    destruct v; auto; try omega.
+    destruct (a == m); subst; auto.
+    destruct (lower_mapping_smaller x m); subst; auto.
+    omega.
+  Qed.
 
-    Definition map (x:t V1) : t V2.
-      refine {| get := fun a => match x a with
-                             | None => None
-                             | Some v => Some (f v)
-                             end;
-                max := max x; |}; intros.
-      destruct_with_eqn (x a); eauto.
-      rewrite mapping_finite in Heqo by auto; congruence.
+  Theorem thread_upd_thread_max_shrink : forall (x:t) a,
+      thread_max (thread_upd x a NoProc) <= thread_max x.
+  Proof.
+    simpl; intros.
+    generalize dependent (thread_max x); intros m **.
+    destruct (lt_dec m a); auto.
+    destruct (a == m); subst; auto.
+    destruct (lower_mapping_smaller x m); subst; auto.
+    omega.
+  Qed.
 
-      destruct (max_minimal x); auto.
-      destruct (x (max x)); auto.
-      left; congruence.
-    Defined.
+  Theorem thread_upd_unchanged : forall (x:t) a T (v: proc Op T),
+      a <= thread_max x ->
+      thread_max (thread_upd x a (Proc v)) = thread_max x.
+  Proof.
+  Abort.
 
-    Theorem map_get_match : forall (x:t V1) a,
-        map x a = match x a with
-                  | Some v => Some (f v)
-                  | None => None
-                  end.
-    Proof.
-      simpl; auto.
-    Qed.
+  Theorem past_thread_max_empty : forall (x:t),
+      x (1 + thread_max x) = NoProc.
+  Proof.
+    intros.
+    apply mapping_finite; omega.
+  Qed.
 
-    Theorem map_get_some : forall (x:t V1) a v,
-        x a = Some v ->
-        map x a = Some (f v).
-    Proof.
-      simpl; intros.
-      rewrite H; auto.
-    Qed.
+  Definition thread_empty : t.
+    refine {| thread_get := fun _ => NoProc;
+              thread_max := 0; |}; auto.
+  Defined.
 
-    Theorem map_get_none : forall (x:t V1) a,
-        x a = None ->
-        map x a = None.
-    Proof.
-      simpl; intros.
-      rewrite H; auto.
-    Qed.
+  Theorem empty_is_empty : forall a,
+      thread_empty a = NoProc.
+  Proof.
+    simpl; auto.
+  Qed.
 
-    Theorem map_Forall : forall (P: V1 -> Prop) (Q:V2 -> Prop) (x:t V1),
-        Forall P x ->
-        (forall v, P v -> Q (f v)) ->
-        Forall Q (map x).
-    Proof.
-      unfold Forall; simpl; intros.
-      destruct_with_eqn (x a).
-      inversion H1; subst; eauto.
-      congruence.
-    Qed.
+  Theorem thread_empty_not_some : forall a T (v: proc Op T),
+      ~thread_empty a = Proc v.
+  Proof.
+    simpl; auto.
+  Qed.
 
-  End Map_map.
+  Theorem thread_empty_unique : forall (x:t),
+      (forall a, x a = NoProc) ->
+      x = thread_empty.
+  Proof.
+    t.
+  Qed.
+
+  Theorem empty_thread_max :
+    thread_max thread_empty = 0.
+  Proof.
+    t.
+  Qed.
+
+  Definition thread_Forall (P: forall T, proc Op T -> Prop) (ts:t) :=
+    forall tid T (p: proc Op T), ts tid = Proc p -> P _ p.
+
+  Theorem thread_Forall_some : forall P x a T (v: proc Op T),
+      thread_Forall P x ->
+      x a = Proc v ->
+      P _ v.
+  Proof.
+    unfold thread_Forall; eauto.
+  Qed.
+
+  Theorem empty_thread_Forall : forall P,
+      thread_Forall P thread_empty.
+  Proof.
+    unfold thread_Forall; intros.
+    apply thread_empty_not_some in H; contradiction.
+  Qed.
+
+  Theorem thread_Forall_thread_upd_some : forall P ts tid T (p: proc Op T),
+      thread_Forall P ts ->
+      P _ p ->
+      thread_Forall P (thread_upd ts tid (Proc p)).
+  Proof.
+    unfold thread_Forall.
+    t.
+    destruct (tid == tid0); subst;
+      rewrite ?Map.thread_upd_eq, ?Map.thread_upd_ne in * by auto;
+      subst;
+      eauto.
+    invert H1.
+  Qed.
+
+  Theorem thread_Forall_forall : forall (P: forall T, proc Op T -> Prop) (x:t),
+      (forall a T (v: proc _ T), x a = Proc v -> P _ v) ->
+      thread_Forall P x.
+  Proof.
+    unfold thread_Forall; eauto.
+  Qed.
+
+  Theorem thread_Forall_thread_upd_none : forall P x tid,
+      thread_Forall P x ->
+      thread_Forall P (thread_upd x tid NoProc).
+  Proof.
+    unfold thread_Forall.
+    t.
+    destruct (tid == tid0); subst;
+      rewrite ?Map.thread_upd_eq, ?Map.thread_upd_ne in * by auto;
+      subst;
+      eauto.
+    congruence.
+  Qed.
+
+  Definition thread_from_list (l: list {T & proc Op T}) : t.
+    refine {| thread_get := fun a => match List.nth_error l a with
+                                  | Some (existT _ _ p) => Proc p
+                                  | None => NoProc
+                                  end;
+              thread_max := length l - 1; |}.
+    intros.
+    assert (length l <= a) by omega.
+    apply List.nth_error_None in H0.
+    simpl_match; auto.
+    destruct_with_eqn (List.nth_error l (length l - 1)); eauto.
+    destruct s; left; congruence.
+    right.
+    apply List.nth_error_None in Heqo.
+    omega.
+  Defined.
+
+  Local Fixpoint _to_list (x:t) n : list V :=
+    match n with
+    | 0 => nil
+    | S n' => _to_list x n' ++ (x n'::nil)
+    end.
+
+  Definition thread_to_list (x:t) : list V := _to_list x (1 + thread_max x).
+
+  Lemma firstn_map : forall A B (f: A -> B) n (l: list A),
+      List.firstn n (List.map f l) = List.map f (List.firstn n l).
+  Proof.
+    induction n; simpl; intros; auto.
+    destruct l; simpl; eauto.
+    rewrite IHn; auto.
+  Qed.
+
+  Lemma nth_error_nil : forall A n,
+      List.nth_error (@nil A) n = None.
+  Proof.
+    induction n; simpl; eauto.
+  Qed.
+
+  (* TODO: prove this, just for fun (note that it is unused; conversion back
+    to lists is only for extraction purposes) *)
+  Lemma from_list__to_list : forall l n,
+      n <= length l ->
+      _to_list (thread_from_list l) n = List.firstn n (List.map (fun '(existT _ _ p) => Proc p) l).
+  Proof.
+    induction n; intros; auto.
+    cbn [_to_list thread_get thread_from_list].
+    rewrite IHn by omega.
+    rewrite ?firstn_map.
+    clear IHn.
+    fold (lt n (length l)) in H.
+  Admitted.
+
+  Theorem thread_from_list_to_list : forall l,
+      0 < length l ->
+      thread_to_list (thread_from_list l) = List.map (fun '(existT _ _ p) => Proc p) l.
+  Proof.
+    unfold thread_to_list; intros.
+    unfold thread_to_list.
+    rewrite from_list__to_list by (simpl; omega).
+    rewrite List.firstn_all2; auto.
+    rewrite List.map_length.
+    simpl; omega.
+  Qed.
 
 End Map.
 
-Global Opaque Map.get Map.upd Map.empty Map.Forall Map.from_list Map.map.
+Theorem thread_max_eq : forall Op1 Op2 (ts1:threads_state Op1) (ts2:threads_state Op2),
+    (forall tid, ts1 tid = NoProc <-> ts2 tid = NoProc) ->
+    thread_max ts1 = thread_max ts2.
+Proof.
+  (* will do proof by symmetry *)
+  assert (forall V1 V2 (x1:threads_state V1) (x2:threads_state V2),
+             (forall a, x1 a = NoProc <-> x2 a = NoProc) ->
+             thread_max x1 < thread_max x2 -> False).
+  intros.
+  pose proof (@mapping_finite _ x1 (thread_max x2) ltac:(omega)).
+  apply H in H1.
+  destruct (thread_max_minimal x2); try congruence.
+  omega.
 
-Hint Rewrite Map.upd_eq : upd.
-Hint Rewrite Map.upd_ne using solve [ auto ] : upd.
-Hint Rewrite Map.upd_upd_eq : upd.
-Hint Rewrite Map.upd_same_eq using solve [ auto ] : upd.
-Hint Rewrite Map.map_get_none using solve [ auto ] : upd.
-Hint Rewrite Map.empty_max : upd.
+  intros.
+  assert (forall a, ts2 a = NoProc <-> ts1 a = NoProc).
+  split; intuition auto.
+  apply H0; auto.
+  apply H0; auto.
+  pose proof (H _ _ ts1 ts2).
+  pose proof (H _ _ ts2 ts1).
+  intuition auto.
+  omega.
+Qed.
+
+Section Map_map.
+
+  Variable Op1:Type -> Type.
+  Variable Op2:Type -> Type.
+  Variable f:forall T, proc Op1 T -> proc Op2 T.
+
+  Definition thread_map (x:threads_state Op1) : threads_state Op2.
+    refine {| thread_get := fun a => match x a with
+                                  | NoProc => NoProc
+                                  | Proc v => Proc (f v)
+                                  end;
+              thread_max := thread_max x; |}; intros.
+    destruct_with_eqn (x a); eauto.
+    rewrite mapping_finite in Heqm by auto; congruence.
+
+    destruct (thread_max_minimal x); auto.
+    destruct (x (thread_max x)); auto.
+    left; congruence.
+  Defined.
+
+  Theorem thread_map_get_match : forall (x:threads_state Op1) a,
+      thread_map x a = match x a with
+                       | Proc v => Proc (f v)
+                       | NoProc => NoProc
+                       end.
+  Proof.
+    simpl; auto.
+  Qed.
+
+  Theorem map_thread_get_some : forall (x:threads_state Op1) a T (v: proc Op1 T),
+      x a = Proc v ->
+      thread_map x a = Proc (f v).
+  Proof.
+    simpl; intros.
+    rewrite H; auto.
+  Qed.
+
+  Theorem map_thread_get_none : forall (x:threads_state Op1) a,
+      x a = NoProc ->
+      thread_map x a = NoProc.
+  Proof.
+    simpl; intros.
+    rewrite H; auto.
+  Qed.
+
+  Theorem map_thread_Forall : forall (P: forall T, proc Op1 T -> Prop) (Q:forall T, proc Op2 T -> Prop) (x:threads_state Op1),
+      thread_Forall P x ->
+      (forall T v, P T v -> Q T (f v)) ->
+      thread_Forall Q (thread_map x).
+  Proof.
+    unfold thread_Forall; simpl; intros.
+    destruct_with_eqn (x tid).
+    inversion H1; subst; eauto.
+    congruence.
+  Qed.
+
+End Map_map.
+
+Global Opaque
+       thread_get
+       thread_upd
+       thread_empty
+       thread_Forall
+       thread_from_list
+       thread_to_list
+       thread_map.
+
+Arguments thread_empty {Op}.
+
+Hint Rewrite thread_upd_eq : t.
+Hint Rewrite thread_upd_ne using solve [ auto ] : t.
+Hint Rewrite thread_upd_thread_upd_eq : t.
+Hint Rewrite thread_upd_same_eq using solve [ auto ] : t.
+Hint Rewrite map_thread_get_none using solve [ auto ] : t.
+Hint Rewrite empty_thread_max : t.
